## 降幂公式

$$ \sin^2\alpha = \frac 1 2 (1 - \cos 2\alpha) $$

$$ \sin^3\alpha = \frac 1 4 (3\sin\alpha - \sin 3\alpha) $$

$$ \sin^4\alpha = \frac 1 8 (3 - 4\cos 2\alpha + \cos 4\alpha) $$

$$ \sin^{2n}\alpha = \frac 1 {2^{2n - 1}} [\sum_{k = 0}^{n - 1}(-1)^{n + k}C_{2n}^k \cos(2n - 2k)\alpha + \frac 1 2 C_{2n}^n] $$

$$ \sin^{2n + 1}\alpha = \frac 1 {2^{2n}} \sum_{k = 0}^n (-1)^{n + k}C_{2n + 1}^k \sin(2n - 2k + 1)\alpha $$

$$ \cos^2\alpha = \frac 1 2(1 + \cos 2\alpha) $$

$$ \cos^3\alpha = \frac 1 4(3\cos\alpha + \cos 3\alpha) $$

$$ \cos^4\alpha = \frac 1 8(3 + 4\cos 2\alpha + \cos 4\alpha) $$

$$ \cos^{2n}\alpha = \frac 1 {2^{2n - 1}}[\sum_{k = 0}^{n - 1} C_{2n}^k \cos(2n - 2k)\alpha + \frac 1 2 C_{2n}^n] $$

$$ \cos^{2n + 1}\alpha = \frac 1 {2^{2n}}\sum_{k = 0}^n C_{2n + 1}^k \cos(2n - 2k + 1)\alpha $$

以上式中的 $n$ 为正整数。
