## 加法公式

$$ \sin(\alpha \pm \beta) = \sin\alpha \cos\beta \pm \cos\alpha \sin\beta $$

$$ \cos(\alpha \pm \beta) = \cos\alpha \cos\beta \mp \sin\alpha \sin\beta $$

$$ \tan(\alpha \pm \beta) = \frac{\tan\alpha \pm \tan\beta}{1 \mp \tan\alpha \tan\beta} $$

$$ \cot(\alpha \pm \beta) = \frac{\cot\alpha \cot\beta \mp 1}{\cot\beta \pm \cot\alpha} $$

$$ \begin{eqnarray}
\sin(\alpha + \beta + \gamma) &=& \sin\alpha \cos\beta \cos\gamma + \cos\alpha \sin\beta \cos\gamma 
		+ \cos\alpha \cos\beta \sin\gamma - \sin\alpha \sin\beta\sin\gamma \\
	&=& \sin\alpha \sin\beta \sin\gamma(\cot\beta \cot \gamma + \cot\gamma \cot\alpha + \cot\alpha \cot\beta - 1) \\
	&=& \cos\alpha \cos\beta \cos\gamma(\tan\alpha + \tan\beta + \tan\gamma - \tan\alpha \tan\beta \tan \gamma)
\end{eqnarray} $$

$$ \begin{eqnarray}
\cos(\alpha + \beta + \gamma) &=& \cos\alpha \cos\beta \cos\gamma - \cos\alpha \sin\beta \sin\gamma
		- \sin\alpha \cos\beta \sin\gamma - \sin\alpha \sin\beta \cos\gamma \\
	&=& \cos\alpha \cos\beta \cos\gamma (1 - \tan\beta \tan\gamma - \tan\gamma \tan\alpha - \tan\alpha \tan\beta) \\
	&=& - \sin\alpha \sin\beta \sin\gamma (\cot\alpha + \cot\beta + \cot\gamma - \cot\alpha \cot\beta \cot\gamma)
\end{eqnarray} $$

$$ \tan(\alpha + \beta + \gamma) = \frac{\tan\alpha + \tan\beta + \tan\gamma - \tan\alpha \tan\beta \tan\gamma}
{1 - \tan\beta \tan\gamma - \tan\gamma \tan\alpha - \tan\alpha \tan\beta}$$

$$ \cot(\alpha + \beta + \gamma) = \frac{\cot\alpha \cot\beta \cot\gamma - \cot\alpha - \cot\beta - \cot\gamma}
{\cot\beta \cot\gamma + \cot\gamma \cot\alpha + \cot\alpha \cot\beta - 1} $$

